Give constructors and type names the locally nameless treatment

src/Syntax.v
@@ -1,4 +1,4 @@
-From TLC Require Import LibString LibLN.
+From TLC Require Import LibString LibList LibLN.
 From MCore Require Import Tactics.
 
 Module Type PAT.
@@ -13,9 +13,19 @@ Module Syntax (P : PAT).
   (************************)
 
   Definition bvar  : Set := nat.
-  Definition tname : Set := var.
-  Definition con   : Set := var.
-  Definition data  : Type := env vars.
+
+  Inductive tname : Set :=
+  | BTName : bvar -> tname
+  | FTName : var  -> tname
+  .
+
+  Inductive con : Set :=
+  | BCon : bvar -> con
+  | FCon : var  -> con
+  .
+
+  Definition data : Type :=
+    list (tname * list con).
 
   Inductive kind : Type :=
   | KiType : kind
@@ -75,46 +85,59 @@ Module Syntax (P : PAT).
      - type-level operations working over terms are suffixed by _t
    *)
 
+
   (* Free variables *)
 
-  Fixpoint ftv (T : type) :=
+  Definition Tfv (T : tname) :=
+    match T with
+    | BTName X => \{}
+    | FTName X => \{X}
+    end
+  .
+
+  Definition Kfv (K : con) :=
+    match K with
+    | BCon X => \{}
+    | FCon X => \{X}
+    end
+  .
+
+  Definition dfv (d : data) : vars :=
+    fold_right
+      (fun '(T,Ks) fvs =>
+         Tfv T \u
+         fold_right (fun con fvs' => Kfv con \u fvs') \{} Ks)
+      \{}
+      d.
+
+  Definition kfv (k : kind) : vars :=
+    match k with
+    | KiType => \{}
+    | KiData d => dfv d
+    end.
+
+  Fixpoint tfv (T : type) : vars :=
     match T with
     | TyBVar X => \{}
     | TyFVar X => \{X}
-    | TyArr T1 T2 => ftv T1 \u ftv T2
-    | TyAll k T' => ftv T'
-    | TyCon ty T => ftv ty
-    | TyData d => \{}
-    end
-  .
+    | TyArr T1 T2 => tfv T1 \u tfv T2
+    | TyAll k T' => kfv k \u tfv T'
+    | TyCon ty T => tfv ty \u Tfv T
+    | TyData d => dfv d
+    end.
 
-  Fixpoint ftv_t (t : term) :=
-    match t with
-    | TmBVar i => \{}
-    | TmFVar x => \{}
-    | TmLam T t' => ftv T \u ftv_t t'
-    | TmApp t1 t2 => ftv_t t1 \u ftv_t t2
-    | TmTyLam k t' => ftv_t t'
-    | TmTyApp t' T => ftv_t t' \u ftv T
-    | TmCon K ty t' => ftv ty \u ftv_t t'
-    | TmType t' => ftv_t t'
-    | TmConDef d ty T t' => ftv ty \u ftv_t t'
-    end
-  .
-
-  Fixpoint fv (t : term) :=
+  Fixpoint fv (t : term) : vars :=
     match t with
     | TmBVar i => \{}
     | TmFVar x => \{x}
-    | TmLam T t' => fv t'
+    | TmLam T t' => tfv T \u fv t'
     | TmApp t1 t2 => fv t1 \u fv t2
-    | TmTyLam k t' => fv t'
-    | TmTyApp t' T => fv t'
-    | TmCon K ty t' => fv t'
+    | TmTyLam k t' => kfv k \u fv t'
+    | TmTyApp t' T => fv t' \u tfv T
+    | TmCon K ty t' => Kfv K \u tfv ty \u fv t'
     | TmType t' => fv t'
-    | TmConDef d ty T t' => fv t'
-    end
-  .
+    | TmConDef d ty T t' => dfv d \u tfv ty \u Tfv T \u fv t'
+    end.
 
   (* Opening *)
   (* Opening a term replaces a bound variable by some other term. *)
@@ -168,15 +191,110 @@ Module Syntax (P : PAT).
   #[export]
    Hint Unfold open : mcore.
 
+
+  Definition Topen (j : nat) (X : tname) (T : tname) :=
+    match T with
+    | BTName i => (If i = j then X else T)
+    | FTName _ => T
+    end.
+
+  Definition Topen_d (j : nat) (X : tname) (d : data) : data :=
+    LibList.map (fun '(T, Ks) => (Topen j X T, Ks)) d.
+
+  Definition Topen_k (j : nat) (X : tname) (k : kind) :=
+    match k with
+    | KiType => k
+    | KiData d => KiData (Topen_d j X d)
+    end.
+
+  Fixpoint Topen_ty (j : nat) (X : tname) (T : type) :=
+    match T with
+    | TyBVar X => T
+    | TyFVar X => T
+    | TyArr T1 T2 => TyArr (Topen_ty j X T1) (Topen_ty j X T2)
+    | TyAll k T' => TyAll (Topen_k j X k) (Topen_ty j X T')
+    | TyCon ty T => TyCon (Topen_ty j X ty) (Topen j X T)
+    | TyData d => TyData (Topen_d j X d)
+    end.
+
+  Fixpoint Topen_t (j : nat) (X : tname) (t : term) :=
+    match t with
+    | TmBVar i => t
+    | TmFVar x => t
+    | TmLam T t' => TmLam (Topen_ty j X T) (Topen_t j X t')
+    | TmApp t1 t2 => TmApp (Topen_t j X t1) (Topen_t j X t2)
+    | TmTyLam k t' => TmTyLam (Topen_k j X k) (Topen_t j X t')
+    | TmTyApp t' T => TmTyApp (Topen_t j X t') (Topen_ty j X T)
+    | TmCon K ty t' => TmCon K (Topen_ty j X ty) (Topen_t j X t')
+    | TmType t' => TmType (Topen_t (S j) X t')
+    | TmConDef d ty T t' =>
+        TmConDef (Topen_d j X d) (Topen_ty j X ty) (Topen j X T) (Topen_t j X t')
+    end.
+
+
+  Definition Kopen (j : nat) (X : con) (K : con) :=
+    match K with
+    | BCon i => (If i = j then X else K)
+    | FCon _ => K
+    end.
+
+  Definition Kopen_d (j : nat) (X : con) (d : data) : data :=
+    LibList.map (fun '(T, Ks) => (T , LibList.map (Kopen j X) Ks)) d.
+
+  Definition Kopen_k (j : nat) (X : con) (k : kind) :=
+    match k with
+    | KiType => k
+    | KiData d => KiData (Kopen_d j X d)
+    end.
+
+  Fixpoint Kopen_ty (j : nat) (X : con) (T : type) :=
+    match T with
+    | TyBVar X => T
+    | TyFVar X => T
+    | TyArr T1 T2 => TyArr (Kopen_ty j X T1) (Kopen_ty j X T2)
+    | TyAll k T' => TyAll (Kopen_k j X k) (Kopen_ty j X T')
+    | TyCon ty T => TyCon (Kopen_ty j X ty) T
+    | TyData d => TyData (Kopen_d j X d)
+    end.
+
+  Fixpoint Kopen_t (j : nat) (X : con) (t : term) :=
+    match t with
+    | TmBVar i => t
+    | TmFVar x => t
+    | TmLam T t' => TmLam (Kopen_ty j X T) (Kopen_t j X t')
+    | TmApp t1 t2 => TmApp (Kopen_t j X t1) (Kopen_t j X t2)
+    | TmTyLam k t' => TmTyLam (Kopen_k j X k) (Kopen_t j X t')
+    | TmTyApp t' T => TmTyApp (Kopen_t j X t') (Kopen_ty j X T)
+    | TmCon K ty t' => TmCon (Kopen j X K) (Kopen_ty j X ty) (Kopen_t j X t')
+    | TmType t' => TmType (Kopen_t j X t')
+    | TmConDef d ty T t' =>
+        TmConDef (Kopen_d j X d) (Kopen_ty j X ty) T (Kopen_t (S j) X t')
+    end.
+
+
   (* Local closure *)
   (* A locally closed term contains no unbound BVars. *)
+
+  Inductive lcT : tname -> Prop :=
+  | LCTName : forall X, lcT (FTName X).
+
+  Inductive lcK : con -> Prop :=
+  | LCKCon : forall X, lcK (FCon X).
+
+  Definition lcd (d : data) : Prop :=
+    Forall (fun '(T, Ks) => lcT T /\ Forall lcK Ks) d.
+
+  Inductive lck : kind -> Prop :=
+  | LCKType : lck KiType
+  | LCKData : forall d, lcd d -> lck (KiData d)
+  .
 
   Inductive lct : type -> Prop :=
   | LCTFVar : forall X, lct (TyFVar X)
   | LCTArr  : forall T1 T2, lct T1 -> lct T2 -> lct (TyArr T1 T2)
-  | LCTAll  : forall L k T, (forall X, X \notin L -> lct ({0 ~> TyFVar X}T)) -> lct (TyAll k T)
-  | LCTCon  : forall ty T, lct ty -> lct (TyCon ty T)
-  | LCTData : forall d, lct (TyData d)
+  | LCTAll  : forall L k T, lck k -> (forall X, X \notin L -> lct ({0 ~> TyFVar X}T)) -> lct (TyAll k T)
+  | LCTCon  : forall ty T, lct ty -> lcT T -> lct (TyCon ty T)
+  | LCTData : forall d, lcd d -> lct (TyData d)
   .
   #[export]
    Hint Constructors lct : mcore.
@@ -185,11 +303,11 @@ Module Syntax (P : PAT).
   | LCFVar   : forall x, lc (TmFVar x)
   | LCAbs    : forall L t T, lct T -> (forall x, x \notin L -> lc ([0 ~> TmFVar x]t)) -> lc (TmLam T t)
   | LCApp    : forall t1 t2, lc t1 -> lc t2 -> lc (TmApp t1 t2)
-  | LCTyLam  : forall L k t, (forall X, X \notin L -> lc ([{0 ~> TyFVar X}] t)) -> lc (TmTyLam k t)
+  | LCTyLam  : forall L k t, lck k -> (forall X, X \notin L -> lc ([{0 ~> TyFVar X}] t)) -> lc (TmTyLam k t)
   | LCTyApp  : forall t T, lc t -> lct T -> lc (TmTyApp t T)
-  | LCCon    : forall K T t, lc t -> lct T -> lc (TmCon K T t)
-  | LCType   : forall t, lc t -> lc (TmType t)
-  | LCConDef : forall d ty T t, lc t -> lct ty -> lc (TmConDef d ty T t)
+  | LCCon    : forall K T t, lcK K ->  lct T -> lc t -> lc (TmCon K T t)
+  | LCType   : forall L t, (forall X, X \notin L -> lc (Topen_t 0 (FTName X) t)) -> lc (TmType t)
+  | LCConDef : forall L d ty T t, lcd d -> lct ty -> lcT T -> (forall X, X \notin L -> lc (Kopen_t 0 (FCon X) t)) -> lc (TmConDef d ty T t)
   .
   #[export]
    Hint Constructors lc : mcore.
@@ -255,7 +373,7 @@ Module Syntax (P : PAT).
   | BindCon   : data -> type -> tname -> binding
   | BindTVar  : kind -> binding
   | BindVar   : type -> binding
-  | BindMatch : match_assum -> binding
+  (* | BindMatch : match_assum -> binding *)
   .
 
   Definition env := env binding.
@@ -276,9 +394,12 @@ Module Syntax (P : PAT).
     let B := gather_vars_with (fun x : var => \{x}) in
     let C := gather_vars_with (fun x : env => dom x) in
     let D := gather_vars_with (fun x : term => fv x) in
-    let E := gather_vars_with (fun x : term => ftv_t x) in
-    let F := gather_vars_with (fun x : type => ftv x) in
-    constr:(A \u B \u C \u D \u E \u F).
+    let E := gather_vars_with (fun x : type => tfv x) in
+    let F := gather_vars_with (fun x : kind => kfv x) in
+    let G := gather_vars_with (fun x : data => dfv x) in
+    let H := gather_vars_with (fun x : con => Kfv x) in
+    let I := gather_vars_with (fun x : tname => Tfv x) in
+    constr:(A \u B \u C \u D \u E \u F \u G \u H \u I).
 
   Ltac pick_fresh x :=
     let L := gather_vars in (pick_fresh_gen L x).
@@ -331,13 +452,13 @@ Module Syntax (P : PAT).
 
   Lemma tsubst_fresh :
     forall X T U,
-      X \notin ftv T ->
+      X \notin tfv T ->
       {X => U}T = T.
   Proof. introv Hfv ; solve_eq T. Qed.
 
   Lemma tsubst_intro :
     forall X T U,
-      X \notin (ftv T) ->
+      X \notin (tfv T) ->
       lct U ->
       {0 ~> U} T = {X => U}({0 ~> TyFVar X}T).
   Proof.
@@ -385,6 +506,22 @@ Module Syntax (P : PAT).
     introv Heq. gen i J. solve_eq t ; inverts* Heq.
   Qed.
 
+  Lemma open_Topen_rec :
+    forall i u J V t,
+      [i ~> u](Topen_t J V t) = Topen_t J V t ->
+      [i ~> u]t = t.
+  Proof.
+    introv Heq. gen i J. solve_eq t ; inverts* Heq.
+  Qed.
+
+  Lemma open_Kopen_rec :
+    forall i u J V t,
+      [i ~> u](Kopen_t J V t) = Kopen_t J V t ->
+      [i ~> u]t = t.
+  Proof.
+    introv Heq. gen i J. solve_eq t ; inverts* Heq.
+  Qed.
+
   Lemma open_lc :
     forall k u t,
       lc t ->
@@ -397,6 +534,12 @@ Module Syntax (P : PAT).
         auto.
     - pick_fresh X.
       rewrite open_topen_neq with (J := 0) (V := TyFVar X);
+        auto.
+    - pick_fresh X.
+      rewrite open_Topen_rec with (J := 0) (V := FTName X);
+        auto.
+    - pick_fresh X.
+      rewrite open_Kopen_rec with (J := 0) (V := FCon X);
         auto.
   Qed.
 
@@ -446,7 +589,7 @@ Module Syntax (P : PAT).
 
   Lemma tsubst_t_fresh :
     forall X t U,
-      X \notin ftv_t t ->
+      X \notin fv t ->
       [{X => U}]t = t.
   Proof.
     introv Hfv.
@@ -455,7 +598,7 @@ Module Syntax (P : PAT).
 
   Lemma tsubst_t_intro :
     forall X U t,
-      X \notin (ftv_t t) ->
+      X \notin fv t ->
       lct U ->
       [{0 ~> U}]t = [{X => U}] ([{0 ~> TyFVar X}]t).
   Proof.
@@ -473,7 +616,7 @@ Module Syntax (P : PAT).
     solve_eq t ; inverts* Heq.
   Qed.
 
-  Lemma topen_t_rec :
+  Lemma topen_t_neq :
     forall I J T U t,
       I <> J ->
       [{I ~> T}] ([{J ~> U}] t) = [{J ~> U}] t ->
@@ -481,6 +624,42 @@ Module Syntax (P : PAT).
   Proof.
     introv Hneq Heq. gen I J.
     solve_eq t ; inverts* Heq; eauto using topen_neq.
+  Qed.
+
+  Lemma topen_Topen_rec :
+    forall i j T U X,
+      {i ~> T} (Topen_ty j (FTName X) U) = Topen_ty j (FTName X) U ->
+      {i ~> T}U = U.
+  Proof.
+    introv Heq. gen i.
+    solve_eq U ; inverts* Heq.
+  Qed.
+
+  Lemma topen_t_Topen_rec :
+    forall n T t X,
+      [{n ~> T}] (Topen_t 0 (FTName X) t) = Topen_t 0 (FTName X) t ->
+      [{n ~> T}]t = t.
+  Proof.
+    introv Heq. generalize dependent 0. gen n.
+    solve_eq t ; inverts* Heq ; apply* topen_Topen_rec.
+  Qed.
+
+  Lemma topen_Kopen_rec :
+    forall i j T U X,
+      {i ~> T} (Kopen_ty j (FCon X) U) = Kopen_ty j (FCon X) U ->
+      {i ~> T}U = U.
+  Proof.
+    introv Heq. gen i.
+    solve_eq U ; inverts* Heq.
+  Qed.
+
+  Lemma topen_t_Kopen_rec :
+    forall n T t X,
+      [{n ~> T}] (Kopen_t 0 (FCon X) t) = Kopen_t 0 (FCon X) t ->
+      [{n ~> T}]t = t.
+  Proof.
+    introv Heq. generalize dependent 0. gen n.
+    solve_eq t ; inverts* Heq ; apply* topen_Kopen_rec.
   Qed.
 
   Lemma topen_t_lc :
@@ -492,12 +671,16 @@ Module Syntax (P : PAT).
     solve_eq Hlc ; try rewrite~ topen_lct.
     - pick_fresh_gen L x. apply* topen_open_rec.
     - pick_fresh_gen L x.
-      rewrite* (@topen_t_rec (S n) 0 T (TyFVar x)).
+      rewrite* (@topen_t_neq (S n) 0 T (TyFVar x)).
+    - pick_fresh_gen L x.
+      apply* topen_t_Topen_rec.
+    - pick_fresh_gen L x.
+      apply* topen_t_Kopen_rec.
   Qed.
 
   Lemma topen_t_subst_comm :
     forall X x t1 t2,
-      X \notin ftv_t t2 ->
+      X \notin fv t2 ->
       lc t2 ->
       [{0 ~> TyFVar X}] ([x => t2]t1) = [x => t2]([{0 ~> TyFVar X}] t1).
   Proof.
@@ -512,12 +695,12 @@ Module Syntax (P : PAT).
 
   Lemma topen_notin :
     forall T X Y,
-      X \notin ftv ({0 ~> TyFVar Y}T) ->
-      X \notin ftv T.
+      X \notin tfv ({0 ~> TyFVar Y}T) ->
+      X \notin tfv T.
   Proof.
     introv Hnin. generalize dependent 0.
-    induction T; intros; simpls*.
-    apply notin_union_r in Hnin as (Hnin1 & Hnin2) ; eauto.
+    induction T; intros; simpls* ;
+      apply notin_union_r in Hnin as (Hnin1 & Hnin2) ; eauto.
   Qed.
 
   Lemma topen_t_tsubst_comm :
